aneris/examples/reliable_communication/lib/repdb/proof/leader/proof_of_proxy.v
@@ -62,50 +62,58 @@ Section Client_Proxy_Proof.
         {{{ RET #();
            ∃ (h hf : wrlog) (a: write_event), Q a h hf }}})%I.
 
-  Lemma write_spec_internal_holds A ip (reqh : val) :
+  Lemma write_spec_internal_holds {MTR:MTS_resources} A ip γ lk (reqh : val) :
     Global_Inv γL γM N -∗
     fixed A -∗
     DB_addr ⤇ srv_si -∗
-    @make_request_spec _ _ _ _ MTC ip reqh -∗
+    @make_request_spec _ _ _ _ MTC _ -∗
+    is_lock (DB_InvName.@"leader") ip γ lk
+            (MTSCanRequest ip reqh) -∗
     write_spec_internal ip
       (λ: "k" "v",
-         match: reqh (InjL ("k", "v")) with
-           InjL "_u" => #()
-         | InjR "_abs" => assert: #false
-         end).
+       match: (λ: "req",
+                 acquire lk ;;
+                 let: "res" := make_request reqh "req" in release lk ;; "res")%V
+                (InjL ("k", "v")) with
+         InjL "_u" => #()
+       | InjR "_abs" => assert: #false
+       end).
   Proof.
-    iIntros "#Hinv #HA #Hsi #Hspec".
+    iIntros "#Hinv #HA #Hsi #Hspec #Hlk".
     rewrite /write_spec_internal.
     iIntros (E k v P Q HE Hkeys) "!# #Hviewshift".
     iIntros (Φ) "!#".
     iIntros "HP HΦ".
     wp_pures.
-    wp_apply ("Hspec" with "[HP]").
-    Unshelve.
-    3:{ simplify_eq /=. left. exact (E, (k, v.(SV_val)), (P, Q)). }
-    iSplit.
-    - iPureIntro.
-      simplify_eq /=.
-      assert (s_valid_val DB_serialization v) as Hs by (apply v.(SV_ser)).
-      eexists _. left. split; first done.
-      exists #k, v . split; first done. split; last done.
-      simplify_eq /=. by eexists _.
-    - simplify_eq /=.
-      rewrite /ReqPre. iFrame "#". iLeft.
-      iExists E, k, v, P, Q.
-      do 4 (iSplit; first done).
-      iFrame "#∗".
-    - iIntros (repd repv) "Hpost".
-      simplify_eq /=.
-      rewrite /ReqPost.
-      iDestruct "Hpost" as "[Hpost|Habs]".
-      -- iDestruct "Hpost" as (E0 k0 v0 P0 Q0 Hinl) "Hpost".
-         iDestruct "Hpost" as (a_new h hf Hrepd ->) "Hpost".
-         wp_pures.
-         iApply "HΦ".
-         inversion Hinl.
-         eauto with iFrame.
-      -- by iDestruct "Habs" as (k0 w0 q0 Hinr) "_".
+    wp_apply (acquire_spec with "Hlk").
+    iIntros (w) "(->&Hlocked&Hreq)".
+    wp_pures.
+    wp_apply ("Hspec" with "[$Hreq HP]").
+    { iSplit.
+      - iPureIntro.
+        simplify_eq /=.
+        assert (s_valid_val DB_serialization v) as Hs by (apply v.(SV_ser)).
+        eexists _. left. split; first done.
+        exists #k, v . split; first done. split; last done.
+        simplify_eq /=. by eexists _.
+      - simplify_eq /=.
+        rewrite /ReqPre. iFrame "#". iLeft.
+        iExists E, k, v, P, Q.
+        do 4 (iSplit; first done).
+        iFrame "#∗". }
+    iIntros (repd repv) "[Hreq Hpost]".
+    wp_pures.
+    wp_apply (release_spec with "[$Hlk $Hlocked $Hreq]").
+    iIntros (w) "->".
+    wp_pures.
+    iDestruct "Hpost" as "[Hpost|Habs]".
+    - iDestruct "Hpost" as (E0 k0 v0 P0 Q0 Hinl) "Hpost".
+      iDestruct "Hpost" as (a_new h hf Hrepd ->) "Hpost".
+      wp_pures.
+      iApply "HΦ".
+      inversion Hinl.
+      eauto with iFrame.
+    - by iDestruct "Habs" as (k0 w0 q0 Hinr) "_".
   Qed.
 
   Definition read_spec_internal (ip : ip_address)
@@ -120,56 +128,69 @@ Section Client_Proxy_Proof.
          (∃ a, ⌜vo = SOMEV (we_val a)⌝ ∗ ⌜wo = Some a⌝))
     }}}%I.
 
-  Lemma read_spec_internal_holds A ip (reqh : val) :
+  Lemma read_spec_internal_holds {MTR:MTS_resources} A ip γ lk (reqh : val) :
     Global_Inv γL γM N -∗
     fixed A -∗
     DB_addr ⤇ srv_si -∗
-    @make_request_spec _ _ _ _ MTC ip reqh -∗
+    @make_request_spec _ _ _ _ MTC _ -∗
+    is_lock (DB_InvName.@"leader") ip γ lk
+            (MTSCanRequest ip reqh) -∗
     ∀ (k : Key) (q : Qp) (h : option write_event),
     read_spec_internal ip
       (λ: "k",
-         match: reqh (InjR "k") with InjL "_abs" => assert: #false | InjR "r" => "r" end)
+         match: (λ: "req",
+                   acquire lk ;;
+                   let: "res" := make_request reqh "req" in release lk ;; "res")%V
+                  (InjR "k") with
+           InjL "_abs" => assert: #false
+         | InjR "r" => "r"
+         end)
            k q h.
   Proof.
-    iIntros "#Hinv #HA #Hsi #Hspec".
+    iIntros "#Hinv #HA #Hsi #Hspec #Hlk".
     iIntros (k q h).
     rewrite /read_spec_internal.
     iIntros (Hkeys Φ) "!#".
     iIntros "Hk HΦ".
     wp_pures.
-    wp_apply ("Hspec" with "[Hk]").
-    Unshelve. 3:{ simplify_eq /=. right. done. }
-    iSplit.
-    - iPureIntro.
-      simplify_eq /=.
-      eapply sum_is_ser_valid.
-      simplify_eq /=. simpl.
-      rewrite /sum_is_ser.
-      eexists _, _. by right.
-    - simplify_eq /=.
-      rewrite /ReqPre. iFrame "#". iRight.
-      iExists _, _, _. by iFrame.
-    - iIntros (repd repv) "Hpost".
-      simplify_eq /=.
-      rewrite /ReqPost.
-      iDestruct "Hpost" as "[Habs|Hpost]".
-      -- by iDestruct "Habs" as (E k0 v0 P0 Q0 Habs) "d".
-      -- iDestruct "Hpost" as (k0 w0 q0 Hinr) "Hpost".
-         iDestruct "Hpost" as (vo Hrepd ->) "(Hmem & Hpost)".
-         wp_pures.
-         iApply "HΦ".
-         inversion Hinr.
-         iFrame.
+    wp_apply (acquire_spec with "Hlk").
+    iIntros (v) "(->&Hlocked&Hreq)".
+    wp_pures.
+    wp_apply ("Hspec" with "[$Hreq Hk]").
+    { iSplit.
+      - iPureIntro.
+        simplify_eq /=.
+        eapply sum_is_ser_valid.
+        simplify_eq /=. simpl.
+        rewrite /sum_is_ser.
+        eexists _, _. by right.
+      - simplify_eq /=.
+        rewrite /ReqPre. iFrame "#". iRight.
+        iExists _, _, _. by iFrame. }
+    iIntros (repd repv) "[Hreq Hpost]".
+    wp_pures.
+    wp_apply (release_spec with "[$Hlk $Hlocked $Hreq]").
+    iIntros (v) "->".
+    wp_pures.
+    iDestruct "Hpost" as "[Habs|Hpost]".
+    - by iDestruct "Habs" as (E k0 v0 P0 Q0 Habs) "d".
+    - iDestruct "Hpost" as (k0 w0 q0 Hinr) "Hpost".
+      iDestruct "Hpost" as (vo Hrepd ->) "(Hmem & Hpost)".
+      wp_pures.
+      iApply "HΦ".
+      inversion Hinr.
+      iFrame.
   Qed.
 
-  Definition init_client_leader_proxy_internal
+  Definition init_client_leader_proxy_internal {MTR : MTS_resources}
     (A : gset socket_address) (sa : socket_address) : iProp Σ :=
     ⌜DB_addr ∈ A⌝ →
     ⌜sa ∉ A⌝ →
     {{{ fixed A ∗
         DB_addr ⤇ srv_si ∗
         sa ⤳ (∅, ∅) ∗
-        (@init_client_proxy_spec _ _ _ _ MTC srv_si) ∗
+        (@init_client_proxy_spec _ _ _ _ MTC _ srv_si) ∗
+        (@make_request_spec _ _ _ _ MTC _) ∗
         free_ports (ip_of_address sa) {[port_of_address sa]} }}}
       init_client_leader_proxy (s_serializer DB_serialization)
                                #sa #DB_addr @[ip_of_address sa]
@@ -177,18 +198,21 @@ Section Client_Proxy_Proof.
         (∀ k q h, read_spec_internal (ip_of_address sa) rd k q h) ∗
           write_spec_internal (ip_of_address sa) wr }}}.
 
-  Lemma init_client_leader_proxy_internal_holds A sa :
+  Lemma init_client_leader_proxy_internal_holds {MTR : MTS_resources} A sa :
     Global_Inv γL γM N ⊢ init_client_leader_proxy_internal A sa.
   Proof.
     iIntros "#Hinv".
     iIntros (HA HnA).
     iIntros (Φ) "!#".
-    iIntros "(#Hf & #Hsi & Hmh & #HClient_proxySpec & Hfp) HΦ".
+    iIntros "(#Hf & #Hsi & Hmh & #HClient_proxySpec & # Hreq_spec & Hfp) HΦ".
     rewrite /init_client_leader_proxy.
     wp_pures.
     wp_apply ("HClient_proxySpec" with "[$Hf $Hfp $Hmh $Hsi][HΦ]"); first done.
     iNext.
-    iIntros (reqh) "#Hspec".
+    iIntros (reqh) "Hreq".
+    wp_pures.
+    wp_apply (newlock_spec (DB_InvName .@ "leader") with "Hreq").
+    iIntros (lk γ) "#Hlk".
     wp_pures.
     iApply "HΦ".
     iSplit.
