aneris/examples/reliable_communication/lib/repdb/repdb_code.v
@@ -130,9 +130,9 @@ Definition start_follower_processing_clients ser : val :=
   (λ: "req", client_request_handler_at_follower "db" "mon" "req").
 
 Definition sync_loop : val :=
-  λ: "db" "log" "mon" "reqf" "n",
+  λ: "db" "log" "mon" "rpc" "n",
   letrec: "aux" "i" :=
-    let: "rep" := "reqf" "i" in
+    let: "rep" := make_request "rpc" "i" in
     let: "k" := Fst (Fst "rep") in
     let: "v" := Snd (Fst "rep") in
     let: "j" := Snd "rep" in
@@ -148,9 +148,7 @@ Definition sync_with_server ser : val :=
   λ: "l_addr" "f2l_addr" "db" "log" "mon",
   let: "rpc" := init_client_proxy req_f2l_ser (rep_l2f_ser ser) "f2l_addr"
                 "l_addr" in
-  let: "reqf" := λ: "req",
-  make_request "rpc" "req" in
-  Fork (sync_loop "db" "log" "mon" "reqf" #0).
+  Fork (sync_loop "db" "log" "mon" "rpc" #0).
 
 Definition init_follower ser : val :=
   λ: "l_addr" "f2l_addr" "f_addr",
